x

src/add_multiply.v
@@ -1,5 +1,5 @@
-From research Require Import base bit circuit multiplier fifo regfile.
 From stdpp Require Import fin finite.
+From research Require Import base bit circuit multiplier fifo regfile.
 
 Notation Maybe := @option.
 
@@ -7,9 +7,10 @@ Inductive Instr :=
 | Add (rd rs1 rs2 : Bit 5)
 | Addi (rd rs1 : Bit 5) (imm : Bit 4)
 | Mul (rd rs1 rs2 : Bit 5)
+| Nop
 | Unknown.
 
-Instance defaultInstr : Default Instr := Unknown.
+Instance defaultInstr : Default Instr := Nop.
 
 Inductive method :=
 | GetIReq
@@ -21,9 +22,10 @@ Inductive state :=
 | State__Decode
 | State__Execute.
 
-Inductive implLeak :=
+Inductive implLeakage :=
 | ImplLeak__Pc (l : Bit 32)
 | ImplLeak__Add
+| ImplLeak__Nop
 | ImplLeak__Mul (a : Bit 4).
 
 Instance state__EqDecision : EqDecision state.
@@ -31,108 +33,114 @@ Proof.
   solve_decision.
 Defined.
 
-Inductive D2E :=
+Inductive DInstr :=
 | DAdd (rd : Bit 5) (v1 v2 : Bit 4)
-| DMul (rd : Bit 5) (v1 v2 : Bit 4).
+| DMul (rd : Bit 5) (v1 v2 : Bit 4)
+| DNop.
 
-Instance defaultD2E : Default D2E := DAdd 0%bv 0%bv 0%bv.
+Instance defaultDInstr : Default DInstr := DNop.
 
 Record AddMultiply :=
-  { addMultiplyM : Multiplier
-  ; addMultiplyRf : RegFile 4 5
-  ; addMultiplyPc : Bit 32
+  { addMultiplyM        : Multiplier
+  ; addMultiplyRf       : RegFile 4 5
+  ; addMultiplyPc       : Bit 32
   ; addMultiplyFromImem : Fifo Instr
-  ; addMultiplyToImem : Fifo (Bit 32)
-  ; addMultiplyD2E : Fifo D2E
-  ; addMultiplySt : state
-  ; addMultiplyTrace : list implLeak
+  ; addMultiplyToImem   : Fifo (Bit 32)
+  ; addMultiplyDInstr   : Fifo DInstr
+  ; addMultiplySt       : state
+  ; addMultiplyTrace    : list implLeakage
   }.
 
 Definition mkAddMultiply :=
   {|
-    addMultiplyM := mkMultiplier;
-    addMultiplyRf := mkRegFile;
-    addMultiplyPc := 0%bv;
-    addMultiplyFromImem := mkFifo;
-    addMultiplyToImem := mkFifo;
-    addMultiplyD2E := mkFifo;
-    addMultiplySt := State__Fetch;
-    addMultiplyTrace := []
+    addMultiplyM         := mkMultiplier;
+    addMultiplyRf        := mkRegFile;
+    addMultiplyPc        := 0%bv;
+    addMultiplyFromImem  := mkFifo;
+    addMultiplyToImem    := mkFifo;
+    addMultiplyDInstr    := mkFifo;
+    addMultiplySt        := State__Fetch;
+    addMultiplyTrace     := []
   |}.
 
 Definition addMultiplyGetIReq :=
-  {{ let%read toImem := addMultiplyToImem in
-     if fifoNotEmpty toImem then
-       let%call d := fifoDeq on addMultiplyToImem in
-       ret d
-     else
-       ret 0%bv
+  {{ let%call d := fifoFirst on addMultiplyToImem in
+     let%call _ := fifoDeq on addMultiplyToImem in
+     ret d
   }}.
 
 Definition addMultiplyGetIResp instr :=
-  {{ let%read fromImem := addMultiplyFromImem in
-     let%read toImem := addMultiplyToImem in
-     when fifoNotFull fromImem && fifoNotFull toImem then
-       let%call _ := fifoEnq instr on addMultiplyFromImem in
-       pass
+  {{ let%call _ := fifoEnq instr on addMultiplyFromImem in
+     pass
   }}.
 
 Definition addMultiplyFetch :=
-  {{ let%read pc := addMultiplyPc in
-     let%read toImem := addMultiplyToImem in
-     when fifoNotFull toImem then
+  guard
+    {{ fun st => bool_decide (st.(addMultiplySt) = State__Fetch) }}
+    {{ let%read pc := addMultiplyPc in
        let%call _ := fifoEnq pc on addMultiplyToImem in
-       let%write addMultiplySt := State__Decode in
+       let%write _ := State__Decode on addMultiplySt in
        pass
-  }}.
+    }}.
 
 Definition addMultiplyDecode :=
-  {{ let%read fromImem := addMultiplyFromImem in
-     let%read toImem   := addMultiplyToImem in
-     let%read d2e      := addMultiplyD2E in
-     let%read rf       := addMultiplyRf in
-     when fifoNotFull d2e && fifoNotEmpty fromImem && fifoNotFull toImem then
-       let%call instr := fifoDeq on addMultiplyFromImem in
+  guard
+    {{ fun st => bool_decide (st.(addMultiplySt) = State__Decode) }}
+    {{ let%read d2e      := addMultiplyDInstr in
+       let%read rf       := addMultiplyRf in
+       let%call instr    := fifoFirst on addMultiplyFromImem in
+       let%call _        := fifoDeq on addMultiplyFromImem in
        match instr with
+       | Nop
        | Unknown =>
-           (* In this case, an unknown instruction is encounteted, could
-              just send a no-op to the execution unit instead. *)
-           let%write addMultiplySt := State__Fetch in pass
+           let%call  _ := fifoEnq DNop on addMultiplyDInstr in
+           let%write _ := State__Execute on addMultiplySt in
+           pass
        | Add rd rs1 rs2 =>
            let v1 := regFileSub rs1 rf in
            let v2 := regFileSub rs2 rf in
-           let%call _ := fifoEnq (DAdd rd v1 v2) on addMultiplyD2E in
-           let%write addMultiplySt := State__Execute in
+           let%call _ := fifoEnq (DAdd rd v1 v2) on addMultiplyDInstr in
+           let%write _ := State__Execute on addMultiplySt in
            pass
        | Mul rd rs1 rs2 =>
            let v1 := regFileSub rs1 rf in
            let v2 := regFileSub rs2 rf in
-           let%call _ := fifoEnq (DMul rd v1 v2) on addMultiplyD2E in
-           let%write addMultiplySt := State__Execute in
+           let%call _ := fifoEnq (DMul rd v1 v2) on addMultiplyDInstr in
+           let%write _ := State__Execute on addMultiplySt in
            pass
        | Addi rd rs1 imm =>
            let v1 := regFileSub rs1 rf in
-           let%call _ := fifoEnq (DAdd rd v1 imm) on addMultiplyD2E in
-           let%write addMultiplySt := State__Execute in
+           let%call _ := fifoEnq (DAdd rd v1 imm) on addMultiplyDInstr in
+           let%write _ := State__Execute on addMultiplySt in
            pass
        end
-  }}.
+    }}.
 
 Definition addMultiplyExecuteAdd rd v1 v2 :=
   {{ let%read pc := addMultiplyPc in
-     let%call _ := fifoDeq on addMultiplyD2E in
+     let%call _ := fifoDeq on addMultiplyDInstr in
      let%call _ := regFileUpd rd (v1 + v2)%bv on addMultiplyRf in
-     let%write addMultiplySt := State__Fetch in
-     let%modify addMultiplyTrace := snoc (ImplLeak__Pc pc) in
-     let%modify addMultiplyTrace := snoc ImplLeak__Add in
-     let%modify addMultiplyPc := fun pc => (pc `+Z` 4)%bv in
+     let%write _ := State__Fetch on addMultiplySt in
+     let%modify _ := snoc (ImplLeak__Pc pc) on addMultiplyTrace in
+     let%modify _ := snoc ImplLeak__Add on addMultiplyTrace in
+     let%modify _ := fun pc => (pc `+Z` 4)%bv on addMultiplyPc in
+     pass
+  }}.
+
+Definition addMultiplyExecuteNop :=
+  {{ let%read pc := addMultiplyPc in
+     let%call _ := fifoDeq on addMultiplyDInstr in
+     let%write _ := State__Fetch on addMultiplySt in
+     let%modify _ := snoc (ImplLeak__Pc pc) on addMultiplyTrace in
+     let%modify _ := snoc ImplLeak__Nop on addMultiplyTrace in
+     let%modify _ := fun pc => (pc `+Z` 4)%bv on addMultiplyPc in
      pass
   }}.
 
 Definition addMultiplyExecuteMul rd v1 v2 :=
-  {{ let%read m := addMultiplyM in
-     let%read pc := addMultiplyPc in
-     match m.(multiplierSt) with
+  {{ let%read pc := addMultiplyPc in
+     let%read st := (multiplierSt ∘ addMultiplyM) in
+     match st with
      | State__Empty =>
          let%call _ := multiplierEnq v1 v2 on addMultiplyM in
          pass
@@ -141,29 +149,26 @@ Definition addMultiplyExecuteMul rd v1 v2 :=
          pass
      | State__Full =>
          let%call v := multiplierDeq on addMultiplyM in
-         match v with
-         | Valid v =>
-             let%call _ := fifoDeq on addMultiplyD2E in
-             let%call _ := regFileUpd rd (truncate v) on addMultiplyRf in
-             let%write addMultiplySt := State__Fetch in
-             let%modify addMultiplyTrace := snoc (ImplLeak__Pc pc) in
-             let%modify addMultiplyTrace := snoc (ImplLeak__Mul v1) in
-             let%modify addMultiplyPc := fun pc => (pc `+Z` 4)%bv in
-             pass
-         | Invalid => pass
-         end
+         let%call _ := fifoDeq on addMultiplyDInstr in
+         let%call _ := regFileUpd rd (truncate v) on addMultiplyRf in
+         let%write _ := State__Fetch on addMultiplySt in
+         let%modify _ := snoc (ImplLeak__Pc pc) on addMultiplyTrace in
+         let%modify _ := snoc (ImplLeak__Mul v1) on addMultiplyTrace in
+         let%modify _ := fun pc => (pc `+Z` 4)%bv on addMultiplyPc in
+         pass
      end
   }}.
 
 Definition addMultiplyExecute :=
-  {{ let%read d2e := addMultiplyD2E in
-     when fifoNotEmpty d2e then
-       let instr := fifoFirst d2e in
+  guard
+    {{ fun st => bool_decide (st.(addMultiplySt) = State__Execute) }}
+    {{ let%call instr := fifoFirst on addMultiplyDInstr in
        match instr with
        | DAdd rd v1 v2 => addMultiplyExecuteAdd rd v1 v2
        | DMul rd v1 v2 => addMultiplyExecuteMul rd v1 v2
+       | DNop => addMultiplyExecuteNop
        end
-  }}.
+    }}.
 
 Definition addMultiplyRule :=
   {{ let%read st := addMultiplySt in
@@ -175,56 +180,38 @@ Definition addMultiplyRule :=
   }}.
 
 Instance addMultiplyCircuit : Circuit :=
-  {| circuitInit := mkAddMultiply
-  ; circuitResult m :=
+  {|
+    mkCircuit := mkAddMultiply;
+    circuitResult m :=
       match m with
       | GetIReq => Bit 32
       | _ => unit
-      end
-  ; circuitCall m :=
+      end;
+    circuitCall m :=
       match m with
       | GetIReq => addMultiplyGetIReq
       | GetIResp resp => addMultiplyGetIResp resp
       | Rule => addMultiplyRule
-      end
-  ; circuitTrace := addMultiplyTrace
+      end;
+    circuitTrace := addMultiplyTrace
   |}.
 
 Section example.
-  Definition ms :=
-    [Rule
-     ; GetIReq
-     ; GetIResp (Addi 1%bv 0%bv 3%bv)
-     ; Rule
-     ; Rule
-     ; Rule
-     ; GetIReq
-     ; GetIResp (Addi 2%bv 0%bv 4%bv)
-     ; Rule
-     ; Rule
-     ; Rule
-     ; GetIReq
-     ; GetIResp (Mul 3%bv 1%bv 2%bv)
-     ; Rule
-     ; Rule
-     ; Rule
-     ; Rule
-     ; Rule
-     ; Rule
-     ; Rule
-     ; Rule
-     ; Rule
-     ; GetIReq
-     ; GetIResp (Mul 4%bv 3%bv 2%bv)
-     ; Rule
-     ; Rule
-     ; Rule
-     ; Rule
-     ; Rule
-     ; Rule
-     ; Rule
-     ; Rule
-    ].
+  Definition runCircuit := runCircuit addMultiplyCircuit.
 
-  Eval vm_compute in runCircuit addMultiplyCircuit ms.
+  Example ex0 := mkAddMultiply.
+
+  Eval vm_compute in ex0.
+
+  Example ex1 :=
+    runCircuit
+      [Rule; GetIReq; GetIResp (Addi 1%bv 0%bv 3%bv); Rule;
+       Rule; Rule; GetIReq; GetIResp (Addi 2%bv 0%bv 4%bv);
+       Rule; Rule; Rule; GetIReq; GetIResp (Mul 3%bv 1%bv 2%bv);
+       Rule; Rule; Rule; Rule; Rule; Rule; Rule; Rule; Rule;
+       GetIReq; GetIResp (Mul 4%bv 3%bv 2%bv); Rule; Rule;
+       Rule; Rule; Rule; Rule; Rule; Rule
+      ].
+
+  Eval vm_compute in ex1.
 End example.
