src/action.v
@@ -3,35 +3,64 @@ From research Require Import base.
 Section WithContext.
   Context {s : Type}.
 
-  Definition Action (t : Type) := s -> t * s.
+  (* An action is a guarded state monad. *)
+  Definition Action (t : Type) := s -> option (t * s).
 
-  Definition ret {t} (x : t) : Action t := fun s => (x, s).
+  Definition ret {t} (x : t) : Action t := fun s => Some (x, s).
+
   Definition bind {t1 t2} (m : Action t1) (f : t1 -> Action t2) :=
-    fun r => let (x, s) := m r in (f x) s.
+    fun r =>
+      match m r with
+      | Some (x, s) => (f x) s
+      | None => None
+      end.
 
   Definition fmap {t1 t2} (m : Action t1) (f : t1 -> t2) :=
-    bind m (fun x => ret (f x)).
+    Eval cbv [ bind ret ] in bind m (fun x => ret (f x)).
 
-  Definition pass : Action unit := ret tt.
+  Definition pass : Action unit := Eval cbv [ ret ] in ret tt.
+  Definition fail {t} : Action t := fun _ => None.
 
-  Definition get : Action s := fun s => (s, s).
-  Definition put (x : s) : Action unit := fun _ => (tt, x).
-  Definition modify (f : s -> s) : Action unit := fun s => (tt, f s).
+  Definition get : Action s := fun s => Some (s, s).
+  Definition put (x : s) : Action unit := fun _ => Some (tt, x).
+  Definition modify (f : s -> s) : Action unit := fun s => Some (tt, f s).
 
-  Definition runAction  {a} (m : Action a) (x : s) := m x.
-  Definition runAction1 {a} (m : Action a) := (fst ∘ (runAction (a := a) m)).
-  Definition runAction2 {a} (m : Action a) := (snd ∘ (runAction (a := a) m)).
+  Definition guard {t} (b : s -> bool) (m : Action t) : Action t :=
+    fun s => if b s then m s else fail s.
+
+  Definition runAction {a} (m : Action a) (x : s) := m x.
+
+  Definition runAction1 {a} (m : Action a) :=
+    (option_map fst ∘ (runAction (a := a) m)).
+
+  Definition runAction2 {a} (m : Action a) :=
+    (option_map snd ∘ (runAction (a := a) m)).
 End WithContext.
-
-Global Hint Unfold get put modify bind ret runAction runAction1 runAction2 : core.
 
 Declare Scope action_scope.
 Delimit Scope action_scope with action.
+Local Open Scope action_scope.
 
 Infix ">>=" := bind (at level 60) : action_scope.
 Infix ">>|" := fmap (at level 60) : action_scope.
 
-Notation "'{{' e '}}'" := (e%action : Action _).
+(* Get a field from state *)
+Definition getField {s a} (getter : s -> a) : Action (s := s) a :=
+  get >>= (fun s => ret (getter s)).
+
+(* Run action on field and update state with result *)
+Definition call {s a b}
+  (getter : s -> a)
+  (setter : a -> s -> s)
+  (action : Action (s := a) b) : Action (s := s) b :=
+  get >>= (fun s =>
+             match runAction action (getter s) with
+             | Some (x, s') =>
+                 put (setter s' s) >>= (fun _ => ret x)
+             | None => fail
+             end).
+
+Notation "'{{' e '}}'" := (e%action).
 
 Notation "'let%bind' x ':=' e1 'in' e2" :=
   (e1 >>= (fun x => e2))%action
@@ -41,23 +70,27 @@ Notation "'let%map' x ':=' e1 'in' e2" :=
   (e1 >>| (fun x => e2))%action
     (at level 100, x pattern, e2 at level 200, right associativity) : action_scope.
 
-Notation "'let%read' x ':=' e1 'in' e2" :=
-  (get >>| e1 >>= (fun x => e2))%action
+Notation "'let%read' x ':=' proj 'in' e2" :=
+  (getField proj >>= (fun x => e2))%action
     (at level 100, x at next level, e2 at level 200, right associativity) : action_scope.
 
-Notation "'let%write' x ':=' e1 'in' e2" :=
-  (modify (set x (fun _ => e1)) >>= (fun _ => e2))%action
-    (at level 100, x at next level, e2 at level 200, right associativity) : action_scope.
+(* TODO knwabueze: Maybe make %write and %modify return the prior value?? *)
+Notation "'let%write' '_' ':=' e1 'on' proj 'in' e2" :=
+  (modify (fun s => s <| proj := e1 |>) >>= (fun _ => e2))%action
+    (at level 100, proj at next level, e2 at level 200, right associativity) : action_scope.
 
-Notation "'let%modify' x ':=' e1 'in' e2" :=
-  (modify (set x e1) >>= (fun _ => e2))%action
-    (at level 100, x at next level, e2 at level 200, right associativity) : action_scope.
+Notation "'let%modify' '_' ':=' e1 'on' proj 'in' e2" :=
+  (modify (fun s => s <| proj ::= e1 |>) >>= (fun _ => e2))%action
+    (at level 100, proj at next level, e2 at level 200, right associativity) : action_scope.
 
-Notation "'let%call' x ':=' e1 'on' field 'in' e2" :=
-  (get >>= (fun s =>
-              let (x, s') := runAction e1 (field s) in
-              put (set field (fun _ : _ => s') s) >>= (fun _ => e2)))%action
-    (at level 100, x pattern, e1 at next level, field at next level,
+Notation "'let%call' x ':=' e1 'on' proj 'in' e2" :=
+  (call proj (fun v s => s <| proj := v |>) e1 >>= (fun x => e2))%action
+    (at level 100, x pattern, e1 at next level, proj at next level,
       e2 at level 200, right associativity) : action_scope.
 
 Notation " 'when' c 'then' e " := (if c then e else pass) (at level 200) : action_scope.
+
+Global Hint Unfold get put modify fmap bind ret fail pass guard : core.
+Global Hint Unfold runAction runAction1 runAction2 : core.
+Global Hint Unfold getField call : core.
+Global Hint Unfold option_map from_option : core.
