src/fifo.v
@@ -4,37 +4,38 @@ Section WithContext.
   Context (a : Type) `{Default a}.
 
   Record Fifo := { fifoContents : Maybe a }.
-
   Definition mkFifo := {| fifoContents := Invalid |}.
 
   Definition fifoNotEmpty s := bool_decide (s.(fifoContents) <> Invalid).
+
   Definition fifoNotFull s := bool_decide (s.(fifoContents) = Invalid).
 
-  Definition fifoEnq in__a :=
-    {{ let%read first := fifoContents in
-       when decide (first = Invalid) then
-         let%write fifoContents := Valid in__a in
+  Definition fifoEnq x1 :=
+    guard
+      {{ fifoNotFull }}
+      {{ let%write _ := Valid x1 on fifoContents in
          pass
-    }}.
+      }}.
 
   Definition fifoDeq :=
-    {{ let%read first := fifoContents in
-       let%write fifoContents := Invalid in
-       match first with
-       | Valid x => ret x
-       | Invalid => ret δ
-       end
-    }}.
+    guard
+      {{ fifoNotEmpty }}
+      {{ let%write _ := Invalid on fifoContents in
+         pass
+      }}.
 
-  Definition fifoFirst s :=
-    match s.(fifoContents) with
-    | Valid x => x
-    | Invalid => δ
-    end.
+  Definition fifoFirst :=
+    guard
+      {{ fifoNotEmpty }}
+      {{ let%read x := fifoContents in
+         match x with
+         | Valid x => ret x
+         | Invalid => ret δ
+         end
+      }}.
 End WithContext.
 
 Arguments mkFifo {_}.
 Arguments fifoEnq {_} (_ _).
-Arguments fifoDeq {_ _} (_).
-Arguments fifoNotEmpty {_} (_).
-Arguments fifoNotFull {_} (_).
+Arguments fifoDeq {_} (_).
+Arguments fifoFirst {_ _} (_).
